Hashmap/AssocList/Map.lean
@@ -1,0 +1,126 @@
+/-
+Copyright (c) 2024 Lean FRO, LLC. All rights reserved.
+Released under Apache 2.0 license as described in the file LICENSE.
+Authors: Markus Himmel
+-/
+import Hashmap.AssocList.Basic
+
+namespace Lean
+
+def AssocListMap (α : Type u) [BEq α] (β : Type v) :=
+  { l : AssocList α β // l.WF }
+
+theorem AssocListMap.ext [BEq α] {l l' : AssocListMap α β} : l.1 = l'.1 → l = l' := by
+  cases l; cases l'; rintro rfl; rfl
+
+namespace AssocListMap
+
+def nil [BEq α] : AssocListMap α β :=
+  ⟨AssocList.nil, AssocList.WF_nil⟩
+
+def findEntry? [BEq α] (a : α) : AssocListMap α β → Option (α × β) :=
+  fun l => l.1.findEntry? a
+
+@[simp]
+theorem findEntry?_nil [BEq α] {a : α} : (nil : AssocListMap α β).findEntry? a = none :=
+  AssocList.findEntry?_nil
+
+theorem findEntry?_eq_of_beq [BEq α] [EquivBEq α] {l : AssocListMap α β} {a a' : α} (h : a == a') :
+    l.findEntry? a = l.findEntry? a' :=
+  AssocList.findEntry?_eq_of_beq h
+
+def find? [BEq α] (a : α) : AssocListMap α β → Option β :=
+  fun l => l.1.find? a
+
+@[simp]
+theorem find?_nil [BEq α] {a : α} : (nil : AssocListMap α β).find? a = none :=
+  AssocList.find?_nil
+
+theorem find?_eq_findEntry? [BEq α] {l : AssocListMap α β} {a : α} :
+    l.find? a = (l.findEntry? a).map (·.2) :=
+  AssocList.find?_eq_findEntry?
+
+theorem find?_eq_of_beq [BEq α] [EquivBEq α] {l : AssocListMap α β} {a a' : α} (h : a == a') :
+    l.find? a = l.find? a' :=
+  AssocList.find?_eq_of_beq h
+
+def findKey? [BEq α] (a : α) : AssocListMap α β → Option α :=
+  fun l => l.1.findKey? a
+
+@[simp]
+theorem findKey?_nil [BEq α] {a : α} : (nil : AssocListMap α β).findKey? a = none :=
+  AssocList.findKey?_nil
+
+theorem findKey?_eq_findEntry? [BEq α] {l : AssocListMap α β} {a : α} :
+    l.findKey? a = (l.findEntry? a).map (·.1) :=
+  AssocList.findKey?_eq_findEntry?
+
+theorem findKey?_eq_of_beq [BEq α] [EquivBEq α] {l : AssocListMap α β} {a a' : α} (h : a == a') :
+    l.findKey? a = l.findKey? a' :=
+  AssocList.findKey?_eq_of_beq h
+
+def contains [BEq α] (a : α) : AssocListMap α β → Bool :=
+  fun l => l.1.contains a
+
+@[simp]
+theorem contains_nil [BEq α] {a : α} : (nil : AssocListMap α β).contains a = false :=
+  AssocList.contains_nil
+
+theorem contains_eq_isSome_findEntry? [BEq α] {l : AssocListMap α β} :
+    l.contains a = (l.findEntry? a).isSome :=
+  AssocList.contains_eq_isSome_findEntry?
+
+theorem contains_eq_isSome_find? [BEq α] {l : AssocListMap α β} :
+    l.contains a = (l.find? a).isSome :=
+  AssocList.contains_eq_isSome_find?
+
+theorem contains_eq_isSome_findKey? [BEq α] {l : AssocListMap α β} :
+    l.contains a = (l.findKey? a).isSome :=
+  AssocList.contains_eq_isSome_findKey?
+
+theorem contains_eq_of_beq [BEq α] [EquivBEq α] {l : AssocListMap α β} {a b : α} (h : a == b) :
+    l.contains a = l.contains b :=
+  AssocList.contains_eq_of_beq h
+
+theorem contains_of_beq [BEq α] [EquivBEq α] {l : AssocListMap α β} {a b : α} (hla : l.contains a)
+    (hab : a == b) : l.contains b :=
+  AssocList.contains_of_beq hla hab
+
+/- Skipping findEntry, findKey, find for now. -/
+
+/- Skipping replace and cons (with proof arguments) for now. -/
+
+def erase [BEq α] [EquivBEq α] (a : α) : AssocListMap α β → AssocListMap α β :=
+  fun l => ⟨l.1.erase a, AssocList.WF_erase l.2⟩
+
+@[simp]
+theorem erase_nil [BEq α] [EquivBEq α] {a : α} : (nil : AssocListMap α β).erase a = nil :=
+  AssocListMap.ext <| AssocList.erase_nil (a := a)
+
+@[simp]
+theorem findEntry?_erase_self [BEq α] [EquivBEq α] {l : AssocListMap α β} {k : α} :
+    (l.erase k).findEntry? k = none :=
+  AssocList.findEntry?_erase_self l.2
+
+theorem findEntry?_erase_of_beq [BEq α] [EquivBEq α] {l : AssocListMap α β} {k a : α} (h : k == a) :
+    (l.erase k).findEntry? a = none :=
+  AssocList.findEntry?_erase_of_beq l.2 h
+
+theorem findEntry?_erase_of_false [BEq α] [EquivBEq α] {l : AssocListMap α β} {k a : α}
+    (h : (k == a) = false) : (l.erase k).findEntry? a = l.findEntry? a :=
+  AssocList.findEntry?_erase_of_false h
+
+theorem findEntry?_erase [BEq α] [EquivBEq α] {l : AssocListMap α β} {k a : α} :
+    (l.erase k).findEntry? a = bif k == a then none else l.findEntry? a :=
+  AssocList.findEntry?_erase l.2
+
+/- Skipping findKey?_erase, find?_erase and contains_erase for now. -/
+
+def insert [BEq α] [EquivBEq α] (k : α) (v : β) : AssocListMap α β → AssocListMap α β :=
+  fun l => ⟨l.1.insert k v, AssocList.WF_insert l.2⟩
+
+/- Skipping findEntry?_insert, findKey?_insert, find?_insert and contains_insert for now. -/
+
+end AssocListMap
+
+end Lean
