Hashmap/HashMap.lean
@@ -1,0 +1,55 @@
+/-
+Copyright (c) 2018 Microsoft Corporation. All rights reserved.
+Released under Apache 2.0 license as described in the file LICENSE.
+Authors: Leonardo de Moura, Mario Carneiro, Markus Himmel
+-/
+import Hashmap.AssocList.Map
+import Hashmap.LawfulHashable
+
+namespace Lean
+
+namespace HashMap.Imp
+
+def Buckets (α : Type u) [BEq α] (β : Type v) :=
+  { t : Array (AssocListMap α β) // t.size.isPowerOfTwo }
+
+namespace Buckets
+
+def update [BEq α] (b : Buckets α β) (i : USize) (h : i.toNat < b.1.size) (l : AssocListMap α β) : Buckets α β :=
+  ⟨b.1.uset i l h, by simpa using b.2⟩
+
+@[simp]
+theorem update_size [BEq α] {b : Buckets α β} {i : USize} {h : i.toNat < b.1.size} {l : AssocListMap α β} :
+    (b.update i h l).1.size = b.1.size := by simp [update]
+
+-- Todo: this is insane
+macro_rules
+| `(tactic| get_elem_tactic_trivial) => `(tactic| simpa)
+
+theorem update_get [BEq α] {b : Buckets α β} {i : USize} {h : i.toNat < b.1.size} {l : AssocListMap α β}
+    {j : USize} {hj : j.toNat < b.1.size} :
+    (b.update i h l).1[j] = if i = j then l else b.1[j] := by
+  sorry -- Meh
+
+structure BucketWFAt [BEq α] [Hashable α] [LawfulHashable α] (l : AssocListMap α β)
+    (size : Nat) (index : USize) : Prop where
+  hash_valid : ∀ a, l.contains a → (hash a % size).toNat = i
+
+structure WF [BEq α] [Hashable α] [LawfulHashable α] (b : Buckets α β) : Prop where
+  bucket_wf : ∀ (i : USize) (h : i.toNat < b.1.size), BucketWFAt b.1[i] b.1.size i
+
+theorem WF_update [BEq α] [Hashable α] [LawfulHashable α] {b : Buckets α β} {i : USize} {h : i.toNat < b.1.size}
+    {l : AssocListMap α β} : b.WF → BucketWFAt l b.1.size i → (b.update i h l).WF := by
+  refine fun ⟨h₁⟩ h₂ => ⟨fun j hj => ?_⟩
+  rw [update_get]
+  by_cases h' : i = j
+  · simpa [h'] using h₂
+  · simp [h']
+    apply h₁ j
+  · simpa using hj
+
+end Buckets
+
+end HashMap.Imp
+
+end Lean
